Adding full crt and csr support (#38, #25, #40).

src/riot/RIoT.Core.fst
@@ -27,9 +27,11 @@ open RIoT.Impl
 
 module Ed25519 = Hacl.Ed25519
 
+#set-options "--z3rlimit 4096 --fuel 0 --ifuel 0"
+
 #restart-solver
-#push-options "--z3rlimit 1024 --fuel 0 --ifuel 0"
-let riot
+let riot_pre
+  (h: HS.mem)
 (* Common Inputs *)
   (cdi : B.lbuffer byte_sec 32)
   (fwid: B.lbuffer byte_sec 32)
@@ -40,14 +42,22 @@ let riot
 (* DeviceID CSR Inputs*)
   (deviceIDCSR_ku: key_usage_payload_t)
   (deviceIDCSR_version: datatype_of_asn1_type INTEGER)
-  (s_common:  x509_RDN_x520_attribute_string_t COMMON_NAME  IA5_STRING)
-  (s_org:     x509_RDN_x520_attribute_string_t ORGANIZATION IA5_STRING)
-  (s_country: x509_RDN_x520_attribute_string_t COUNTRY      PRINTABLE_STRING)
+  (deviceIDCSR_s_common:  x509_RDN_x520_attribute_string_t COMMON_NAME  IA5_STRING)
+  (deviceIDCSR_s_org:     x509_RDN_x520_attribute_string_t ORGANIZATION IA5_STRING)
+  (deviceIDCSR_s_country: x509_RDN_x520_attribute_string_t COUNTRY      PRINTABLE_STRING)
 (* AliasKey Crt Inputs*)
+  (aliasKeyCrt_version: x509_version_t)
+  (aliasKeyCrt_serialNumber: datatype_of_asn1_type INTEGER)
+  (aliasKeyCrt_i_common:  x509_RDN_x520_attribute_string_t COMMON_NAME  IA5_STRING)
+  (aliasKeyCrt_i_org:     x509_RDN_x520_attribute_string_t ORGANIZATION IA5_STRING)
+  (aliasKeyCrt_i_country: x509_RDN_x520_attribute_string_t COUNTRY      PRINTABLE_STRING)
+  (aliasKeyCrt_notBefore: datatype_of_asn1_type Generalized_Time)
+  (aliasKeyCrt_notAfter : datatype_of_asn1_type Generalized_Time)
+  (aliasKeyCrt_s_common:  x509_RDN_x520_attribute_string_t COMMON_NAME  IA5_STRING)
+  (aliasKeyCrt_s_org:     x509_RDN_x520_attribute_string_t ORGANIZATION IA5_STRING)
+  (aliasKeyCrt_s_country: x509_RDN_x520_attribute_string_t COUNTRY      PRINTABLE_STRING)
   (aliasKeyCrt_ku: key_usage_payload_t)
   (riot_version: datatype_of_asn1_type INTEGER)
-  (aliasKeyTBS_template_len: size_t)
-  (aliasKeyTBS_template: B.lbuffer byte_pub (v aliasKeyTBS_template_len))
 (* Common Outputs *)
   (aliasKey_pub: B.lbuffer byte_pub 32)
   (aliasKey_priv: B.lbuffer uint8 32)
@@ -57,13 +67,11 @@ let riot
 (* AliasKey Crt Outputs *)
   (aliasKeyCRT_len: size_t)
   (aliasKeyCRT_buf: B.lbuffer byte_pub (v aliasKeyCRT_len))
-: HST.Stack unit
-  (requires fun h ->
-    B.(all_live h [buf cdi;
+: Type0
+=   B.(all_live h [buf cdi;
                    buf fwid;
                    buf deviceID_label;
                    buf aliasKey_label;
-                   buf aliasKeyTBS_template;
                    buf deviceIDCSR_buf;
                    buf aliasKeyCRT_buf;
                    buf aliasKey_pub;
@@ -72,7 +80,6 @@ let riot
                      loc_buffer fwid;
                      loc_buffer deviceID_label;
                      loc_buffer aliasKey_label;
-                     loc_buffer aliasKeyTBS_template;
                      loc_buffer deviceIDCSR_buf;
                      loc_buffer aliasKeyCRT_buf;
                      loc_buffer aliasKey_pub;
@@ -81,20 +88,108 @@ let riot
    valid_hkdf_lbl_len deviceID_label_len /\
    valid_hkdf_lbl_len aliasKey_label_len /\
    (* Pre: DeviceIDCRI template has a valid length *)
-   valid_deviceIDCRI_ingredients deviceIDCSR_version s_common s_org s_country deviceIDCSR_ku /\
+   valid_deviceIDCRI_ingredients
+     deviceIDCSR_version
+     deviceIDCSR_s_common deviceIDCSR_s_org deviceIDCSR_s_country
+     deviceIDCSR_ku /\
    (* Pre: DeviceIDCSR will have a valid length *)
-   valid_deviceIDCSR_ingredients (len_of_deviceIDCRI deviceIDCSR_version s_common s_org s_country deviceIDCSR_ku) /\
+   valid_deviceIDCSR_ingredients
+     (len_of_deviceIDCRI
+       deviceIDCSR_version
+       deviceIDCSR_s_common deviceIDCSR_s_org deviceIDCSR_s_country
+       deviceIDCSR_ku) /\
    (* Pre: `deviceIDCSR_buf` has exact size to write DeviceIDCSR *)
-   v deviceIDCSR_len == length_of_deviceIDCSR (len_of_deviceIDCRI deviceIDCSR_version s_common s_org s_country deviceIDCSR_ku) /\
+   v deviceIDCSR_len == length_of_deviceIDCSR
+                          (len_of_deviceIDCRI
+                            deviceIDCSR_version
+                            deviceIDCSR_s_common deviceIDCSR_s_org deviceIDCSR_s_country
+                            deviceIDCSR_ku) /\
    (* Pre: AliasKeyTBS template has a valid length *)
-   valid_aliasKeyTBS_ingredients aliasKeyTBS_template_len aliasKeyCrt_ku riot_version /\
+   valid_aliasKeyTBS_ingredients
+     aliasKeyCrt_serialNumber
+     aliasKeyCrt_i_common aliasKeyCrt_i_org aliasKeyCrt_i_country
+     aliasKeyCrt_s_common aliasKeyCrt_s_org aliasKeyCrt_s_country
+     aliasKeyCrt_ku
+     riot_version /\
    (* Pre: AliasKeyTBS will have a valid length *)
-   valid_aliasKeyCRT_ingredients (len_of_aliasKeyTBS aliasKeyTBS_template_len aliasKeyCrt_ku riot_version) /\
+   valid_aliasKeyCRT_ingredients
+     (len_of_aliasKeyTBS
+       aliasKeyCrt_serialNumber
+       aliasKeyCrt_i_common aliasKeyCrt_i_org aliasKeyCrt_i_country
+       aliasKeyCrt_s_common aliasKeyCrt_s_org aliasKeyCrt_s_country
+       aliasKeyCrt_ku
+       riot_version) /\
    (* Pre: `aliasKeyCRT_buf` has exact size to write AliasKeyCRT *)
-   v aliasKeyCRT_len == length_of_aliasKeyCRT (len_of_aliasKeyTBS aliasKeyTBS_template_len aliasKeyCrt_ku riot_version)
-   )
-   (ensures fun h0 _ h1 ->
-    (* Post: Modifies *)
+   v aliasKeyCRT_len == length_of_aliasKeyCRT
+                          (len_of_aliasKeyTBS
+                            aliasKeyCrt_serialNumber
+                            aliasKeyCrt_i_common aliasKeyCrt_i_org aliasKeyCrt_i_country
+                            aliasKeyCrt_s_common aliasKeyCrt_s_org aliasKeyCrt_s_country
+                            aliasKeyCrt_ku
+                            riot_version)
+
+#restart-solver
+let riot_post
+  (h0: HS.mem)
+  (r: unit)
+  (h1: HS.mem)
+(* Common Inputs *)
+  (cdi : B.lbuffer byte_sec 32)
+  (fwid: B.lbuffer byte_sec 32)
+  (deviceID_label_len: size_t)
+  (deviceID_label: B.lbuffer byte_sec (v deviceID_label_len))
+  (aliasKey_label_len: size_t)
+  (aliasKey_label: B.lbuffer byte_sec (v aliasKey_label_len))
+(* DeviceID CSR Inputs*)
+  (deviceIDCSR_ku: key_usage_payload_t)
+  (deviceIDCSR_version: datatype_of_asn1_type INTEGER)
+  (deviceIDCSR_s_common:  x509_RDN_x520_attribute_string_t COMMON_NAME  IA5_STRING)
+  (deviceIDCSR_s_org:     x509_RDN_x520_attribute_string_t ORGANIZATION IA5_STRING)
+  (deviceIDCSR_s_country: x509_RDN_x520_attribute_string_t COUNTRY      PRINTABLE_STRING)
+(* AliasKey Crt Inputs*)
+  (aliasKeyCrt_version: x509_version_t)
+  (aliasKeyCrt_serialNumber: datatype_of_asn1_type INTEGER)
+  (aliasKeyCrt_i_common:  x509_RDN_x520_attribute_string_t COMMON_NAME  IA5_STRING)
+  (aliasKeyCrt_i_org:     x509_RDN_x520_attribute_string_t ORGANIZATION IA5_STRING)
+  (aliasKeyCrt_i_country: x509_RDN_x520_attribute_string_t COUNTRY      PRINTABLE_STRING)
+  (aliasKeyCrt_notBefore: datatype_of_asn1_type Generalized_Time)
+  (aliasKeyCrt_notAfter : datatype_of_asn1_type Generalized_Time)
+  (aliasKeyCrt_s_common:  x509_RDN_x520_attribute_string_t COMMON_NAME  IA5_STRING)
+  (aliasKeyCrt_s_org:     x509_RDN_x520_attribute_string_t ORGANIZATION IA5_STRING)
+  (aliasKeyCrt_s_country: x509_RDN_x520_attribute_string_t COUNTRY      PRINTABLE_STRING)
+  (aliasKeyCrt_ku: key_usage_payload_t)
+  (riot_version: datatype_of_asn1_type INTEGER)
+(* Common Outputs *)
+  (aliasKey_pub: B.lbuffer byte_pub 32)
+  (aliasKey_priv: B.lbuffer uint8 32)
+(* DeviceID CSR Outputs *)
+  (deviceIDCSR_len: size_t)
+  (deviceIDCSR_buf: B.lbuffer byte_pub (v deviceIDCSR_len))
+(* AliasKey Crt Outputs *)
+  (aliasKeyCRT_len: size_t)
+  (aliasKeyCRT_buf: B.lbuffer byte_pub (v aliasKeyCRT_len)
+                    { riot_pre
+                        (h0)
+                        (cdi)
+                        (fwid)
+                        (deviceID_label_len) (deviceID_label)
+                        (aliasKey_label_len) (aliasKey_label)
+                        (deviceIDCSR_ku)
+                        (deviceIDCSR_version)
+                        (deviceIDCSR_s_common) (deviceIDCSR_s_org) (deviceIDCSR_s_country)
+                        (aliasKeyCrt_version)
+                        (aliasKeyCrt_serialNumber)
+                        (aliasKeyCrt_i_common) (aliasKeyCrt_i_org) (aliasKeyCrt_i_country)
+                        (aliasKeyCrt_notBefore) (aliasKeyCrt_notAfter)
+                        (aliasKeyCrt_s_common) (aliasKeyCrt_s_org) (aliasKeyCrt_s_country)
+                        (aliasKeyCrt_ku)
+                        (riot_version)
+                        (aliasKey_pub)
+                        (aliasKey_priv)
+                        (deviceIDCSR_len) (deviceIDCSR_buf)
+                        (aliasKeyCRT_len) (aliasKeyCRT_buf) })
+: Type0
+=   (* Post: Modifies *)
      B.(modifies (loc_buffer deviceIDCSR_buf `loc_union`
                   loc_buffer aliasKeyCRT_buf `loc_union`
                   loc_buffer aliasKey_pub    `loc_union`
@@ -113,37 +208,128 @@ let riot
                                                  (B.as_seq h0 deviceID_label) in
      let deviceIDCRI: deviceIDCRI_t = create_deviceIDCRI_spec
                                                                          (deviceIDCSR_version)
-                                                                         (s_common)
-                                                                         (s_org)
-                                                                         (s_country)
+                                                                         (deviceIDCSR_s_common)
+                                                                         (deviceIDCSR_s_org)
+                                                                         (deviceIDCSR_s_country)
                                                                          (deviceIDCSR_ku)
                                                                          (deviceID_pub_seq)
                                                                          in
      let deviceIDCRI_seq = serialize_deviceIDCRI `serialize` deviceIDCRI in
-     let deviceIDCRI_len = len_of_deviceIDCRI deviceIDCSR_version s_common s_org s_country deviceIDCSR_ku in
+     let deviceIDCRI_len = len_of_deviceIDCRI
+                             deviceIDCSR_version
+                             deviceIDCSR_s_common deviceIDCSR_s_org deviceIDCSR_s_country
+                             deviceIDCSR_ku in
      let (* Prf *) _ = lemma_serialize_deviceIDCRI_size_exact deviceIDCRI in
      let deviceIDCSR: deviceIDCSR_t deviceIDCRI_len = sign_and_finalize_deviceIDCSR_spec
                                                                 (deviceID_priv_seq)
                                                                 (deviceIDCRI_len)
                                                                 (deviceIDCRI_seq) in
-     let aliasKeyTBS: aliasKeyTBS_t aliasKeyTBS_template_len = create_aliasKeyTBS_spec
-                                                                         (aliasKeyTBS_template_len)
-                                                                         (B.as_seq h0 aliasKeyTBS_template)
-                                                                         (aliasKeyCrt_ku)
-                                                                         (riot_version)
-                                                                         (B.as_seq h0 fwid)
-                                                                         (deviceID_pub_seq)
-                                                                         (B.as_seq h1 aliasKey_pub)
-                                                                         in
-     let aliasKeyTBS_seq = serialize_aliasKeyTBS aliasKeyTBS_template_len `serialize` aliasKeyTBS in
-     let aliasKeyTBS_len = len_of_aliasKeyTBS aliasKeyTBS_template_len aliasKeyCrt_ku riot_version in
-     let (* Prf *) _ = lemma_serialize_aliasKeyTBS_size_exact aliasKeyTBS_template_len aliasKeyTBS in
+     let aliasKeyTBS: aliasKeyTBS_t = create_aliasKeyTBS_spec
+                                        (aliasKeyCrt_version)
+                                        (aliasKeyCrt_serialNumber)
+                                        (aliasKeyCrt_i_common) (aliasKeyCrt_i_org) (aliasKeyCrt_i_country)
+                                        (aliasKeyCrt_notBefore) (aliasKeyCrt_notAfter)
+                                        (aliasKeyCrt_s_common) (aliasKeyCrt_s_org) (aliasKeyCrt_s_country)
+                                        (aliasKeyCrt_ku)
+                                        (riot_version)
+                                        (B.as_seq h0 fwid)
+                                        (deviceID_pub_seq)
+                                        (B.as_seq h1 aliasKey_pub)
+                                        in
+     let aliasKeyTBS_seq = serialize_aliasKeyTBS `serialize` aliasKeyTBS in
+     let aliasKeyTBS_len = len_of_aliasKeyTBS
+                            aliasKeyCrt_serialNumber
+                            aliasKeyCrt_i_common aliasKeyCrt_i_org aliasKeyCrt_i_country
+                            aliasKeyCrt_s_common aliasKeyCrt_s_org aliasKeyCrt_s_country
+                            aliasKeyCrt_ku
+                            riot_version in
+     let (* Prf *) _ = lemma_serialize_aliasKeyTBS_size_exact aliasKeyTBS in
      let aliasKeyCRT: aliasKeyCRT_t aliasKeyTBS_len = sign_and_finalize_aliasKeyCRT_spec
                                                                 (deviceID_priv_seq)
                                                                 (aliasKeyTBS_len)
                                                                 (aliasKeyTBS_seq) in
      B.as_seq h1 deviceIDCSR_buf == serialize_deviceIDCSR deviceIDCRI_len `serialize` deviceIDCSR /\
-     B.as_seq h1 aliasKeyCRT_buf == serialize_aliasKeyCRT aliasKeyTBS_len `serialize` aliasKeyCRT))
+     B.as_seq h1 aliasKeyCRT_buf == serialize_aliasKeyCRT aliasKeyTBS_len `serialize` aliasKeyCRT)
+
+#restart-solver
+let riot
+(* Common Inputs *)
+  (cdi : B.lbuffer byte_sec 32)
+  (fwid: B.lbuffer byte_sec 32)
+  (deviceID_label_len: size_t)
+  (deviceID_label: B.lbuffer byte_sec (v deviceID_label_len))
+  (aliasKey_label_len: size_t)
+  (aliasKey_label: B.lbuffer byte_sec (v aliasKey_label_len))
+(* DeviceID CSR Inputs*)
+  (deviceIDCSR_ku: key_usage_payload_t)
+  (deviceIDCSR_version: datatype_of_asn1_type INTEGER)
+  (deviceIDCSR_s_common:  x509_RDN_x520_attribute_string_t COMMON_NAME  IA5_STRING)
+  (deviceIDCSR_s_org:     x509_RDN_x520_attribute_string_t ORGANIZATION IA5_STRING)
+  (deviceIDCSR_s_country: x509_RDN_x520_attribute_string_t COUNTRY      PRINTABLE_STRING)
+(* AliasKey Crt Inputs*)
+  (aliasKeyCrt_version: x509_version_t)
+  (aliasKeyCrt_serialNumber: datatype_of_asn1_type INTEGER)
+  (aliasKeyCrt_i_common:  x509_RDN_x520_attribute_string_t COMMON_NAME  IA5_STRING)
+  (aliasKeyCrt_i_org:     x509_RDN_x520_attribute_string_t ORGANIZATION IA5_STRING)
+  (aliasKeyCrt_i_country: x509_RDN_x520_attribute_string_t COUNTRY      PRINTABLE_STRING)
+  (aliasKeyCrt_notBefore: datatype_of_asn1_type Generalized_Time)
+  (aliasKeyCrt_notAfter : datatype_of_asn1_type Generalized_Time)
+  (aliasKeyCrt_s_common:  x509_RDN_x520_attribute_string_t COMMON_NAME  IA5_STRING)
+  (aliasKeyCrt_s_org:     x509_RDN_x520_attribute_string_t ORGANIZATION IA5_STRING)
+  (aliasKeyCrt_s_country: x509_RDN_x520_attribute_string_t COUNTRY      PRINTABLE_STRING)
+  (aliasKeyCrt_ku: key_usage_payload_t)
+  (riot_version: datatype_of_asn1_type INTEGER)
+(* Common Outputs *)
+  (aliasKey_pub: B.lbuffer byte_pub 32)
+  (aliasKey_priv: B.lbuffer uint8 32)
+(* DeviceID CSR Outputs *)
+  (deviceIDCSR_len: size_t)
+  (deviceIDCSR_buf: B.lbuffer byte_pub (v deviceIDCSR_len))
+(* AliasKey Crt Outputs *)
+  (aliasKeyCRT_len: size_t)
+  (aliasKeyCRT_buf: B.lbuffer byte_pub (v aliasKeyCRT_len))
+: HST.Stack unit
+  (requires fun h -> riot_pre
+                        (h)
+                        (cdi)
+                        (fwid)
+                        (deviceID_label_len) (deviceID_label)
+                        (aliasKey_label_len) (aliasKey_label)
+                        (deviceIDCSR_ku)
+                        (deviceIDCSR_version)
+                        (deviceIDCSR_s_common) (deviceIDCSR_s_org) (deviceIDCSR_s_country)
+                        (aliasKeyCrt_version)
+                        (aliasKeyCrt_serialNumber)
+                        (aliasKeyCrt_i_common) (aliasKeyCrt_i_org) (aliasKeyCrt_i_country)
+                        (aliasKeyCrt_notBefore) (aliasKeyCrt_notAfter)
+                        (aliasKeyCrt_s_common) (aliasKeyCrt_s_org) (aliasKeyCrt_s_country)
+                        (aliasKeyCrt_ku)
+                        (riot_version)
+                        (aliasKey_pub)
+                        (aliasKey_priv)
+                        (deviceIDCSR_len) (deviceIDCSR_buf)
+                        (aliasKeyCRT_len) (aliasKeyCRT_buf)
+   )
+   (ensures fun h0 _ h1 -> riot_post
+                        (h0) () (h1)
+                        (cdi)
+                        (fwid)
+                        (deviceID_label_len) (deviceID_label)
+                        (aliasKey_label_len) (aliasKey_label)
+                        (deviceIDCSR_ku)
+                        (deviceIDCSR_version)
+                        (deviceIDCSR_s_common) (deviceIDCSR_s_org) (deviceIDCSR_s_country)
+                        (aliasKeyCrt_version)
+                        (aliasKeyCrt_serialNumber)
+                        (aliasKeyCrt_i_common) (aliasKeyCrt_i_org) (aliasKeyCrt_i_country)
+                        (aliasKeyCrt_notBefore) (aliasKeyCrt_notAfter)
+                        (aliasKeyCrt_s_common) (aliasKeyCrt_s_org) (aliasKeyCrt_s_country)
+                        (aliasKeyCrt_ku)
+                        (riot_version)
+                        (aliasKey_pub)
+                        (aliasKey_priv)
+                        (deviceIDCSR_len) (deviceIDCSR_buf)
+                        (aliasKeyCRT_len) (aliasKeyCRT_buf))
 = HST.push_frame ();
 
 (* Derive DeviceID *)
@@ -168,15 +354,20 @@ let riot
               aliasKey_label;
 
 (* Create DeviceIDCRI *)
-   let deviceIDCRI_len: asn1_TLV_int32_of_type SEQUENCE = len_of_deviceIDCRI deviceIDCSR_version s_common s_org s_country deviceIDCSR_ku in
+   let deviceIDCRI_len: asn1_TLV_int32_of_type SEQUENCE = len_of_deviceIDCRI
+                                                            deviceIDCSR_version
+                                                            deviceIDCSR_s_common
+                                                            deviceIDCSR_s_org
+                                                            deviceIDCSR_s_country
+                                                            deviceIDCSR_ku in
    let deviceIDCRI_buf: B.lbuffer byte_pub (v deviceIDCRI_len) = B.alloca 0x00uy deviceIDCRI_len in
 
    printf "Creating DeviceID Certificate Signing Request Information\n" done;
    create_deviceIDCRI
     (* version   *) deviceIDCSR_version
-                    s_common
-                    s_org
-                    s_country
+                    deviceIDCSR_s_common
+                    deviceIDCSR_s_org
+                    deviceIDCSR_s_country
     (* key usage *) deviceIDCSR_ku
     (* DeviceID  *) deviceID_pub
     (*DeviceIDCRI*) deviceIDCRI_len
@@ -191,18 +382,26 @@ let riot
     (*DeviceIDCSR*) deviceIDCSR_len
                     deviceIDCSR_buf;
 (* Create AliasKeyTBS *)
-  let aliasKeyTBS_len: asn1_TLV_int32_of_type SEQUENCE = len_of_aliasKeyTBS aliasKeyTBS_template_len aliasKeyCrt_ku riot_version in
+  let aliasKeyTBS_len: asn1_TLV_int32_of_type SEQUENCE = len_of_aliasKeyTBS
+                                                           aliasKeyCrt_serialNumber
+                                                           aliasKeyCrt_i_common aliasKeyCrt_i_org aliasKeyCrt_i_country
+                                                           aliasKeyCrt_s_common aliasKeyCrt_s_org aliasKeyCrt_s_country
+                                                           aliasKeyCrt_ku
+                                                           riot_version in
   let aliasKeyTBS_buf: B.lbuffer byte_pub (v aliasKeyTBS_len) = B.alloca 0x00uy aliasKeyTBS_len in
 
   printf "Creating AliasKey Certificate TBS\n" done;
   create_aliasKeyTBS
-    (* FWID      *) fwid
-    (* key usage *) aliasKeyCrt_ku
-    (* version   *) riot_version
+    (aliasKeyCrt_version)
+    (aliasKeyCrt_serialNumber)
+    (aliasKeyCrt_i_common) (aliasKeyCrt_i_org) (aliasKeyCrt_i_country)
+    (aliasKeyCrt_notBefore) (aliasKeyCrt_notAfter)
+    (aliasKeyCrt_s_common) (aliasKeyCrt_s_org) (aliasKeyCrt_s_country)
+    (fwid)
+    (aliasKeyCrt_ku)
+    (riot_version)
     (* DeviceID  *) deviceID_pub
     (* AliasKey  *) aliasKey_pub
-    (* Template  *) aliasKeyTBS_template_len
-                    aliasKeyTBS_template
     (*AliasKeyTBS*) aliasKeyTBS_len
                     aliasKeyTBS_buf;
 
