src/riot/RIoT.X509.AliasKeyTBS.fst
@@ -3,28 +3,40 @@ module RIoT.X509.AliasKeyTBS
 open ASN1.Spec
 open ASN1.Low
 open X509
-// open RIoT.X509.Base
-// include RIoT.X509.FWID
-// include RIoT.X509.CompositeDeviceID
-// include RIoT.X509.Extension
+open RIoT.X509.AliasKeyTBS.Issuer
+open RIoT.X509.AliasKeyTBS.Subject
 open RIoT.X509.AliasKeyTBS.Extensions
 open FStar.Integers
 
 module B32 = FStar.Bytes
 
-open LowParse.Spec.SeqBytes.Base
-open LowParse.Spec.Bytes
+#set-options "--z3rlimit 256 --fuel 0 --ifuel 0"
 
-type aliasKeyTBS_payload_t (header_len: asn1_int32) = {
-(* TEMPLATE of
+type aliasKeyTBS_payload_t = {
+(*
  *       version         [0]  EXPLICIT Version DEFAULT v1,
+ *)
+  aliasKeyTBS_version     : x509_version_t;
+(*
  *       serialNumber         CertificateSerialNumber,
+ *)
+  aliasKeyTBS_serialNumber: datatype_of_asn1_type INTEGER;
+(*
  *       signature            AlgorithmIdentifier,
+ *)
+  aliasKeyTBS_signatureAlg: algorithmIdentifier_t;
+(*
  *       issuer               Name,
+ *)
+  aliasKeyTBS_issuer      : aliasKeyTBS_issuer_t;
+(*
  *       validity             Validity,
+ *)
+ aliasKeyTBS_validity     : x509_validity_t;
+(*
  *       subject              Name,
  *)
-  aliasKeyTBS_template    : B32.lbytes32 header_len;
+  aliasKeyTBS_subject     : aliasKeyTBS_subject_t;
  (*
   *      subjectPublicKeyInfo SubjectPublicKeyInfo
   *)
@@ -36,279 +48,569 @@ type aliasKeyTBS_payload_t (header_len: asn1_int32) = {
                               serialize_aliasKeyTBS_extensions
 }
 
-let aliasKeyTBS_payload_t' (header_len: asn1_int32) = (
-   B32.lbytes32 header_len `tuple2`
-   subjectPublicKeyInfo_t `tuple2`
-   x509_extensions_t_inbound serialize_aliasKeyTBS_extensions
+let aliasKeyTBS_payload_t' = (
+(*
+ *       version         [0]  EXPLICIT Version DEFAULT v1,
+ *)
+  x509_version_t `tuple2`
+(*
+ *       serialNumber         CertificateSerialNumber,
+ *)
+  datatype_of_asn1_type INTEGER `tuple2`
+(*
+ *       signature            AlgorithmIdentifier,
+ *)
+  algorithmIdentifier_t `tuple2`
+(*
+ *       issuer               Name,
+ *)
+  aliasKeyTBS_issuer_t `tuple2`
+(*
+ *       validity             Validity,
+ *)
+  x509_validity_t `tuple2`
+(*
+ *       subject              Name,
+ *)
+  aliasKeyTBS_subject_t `tuple2`
+(*
+ *      subjectPublicKeyInfo SubjectPublicKeyInfo
+ *)
+  subjectPublicKeyInfo_t `tuple2`
+(*
+ *      extensions      [3]  EXPLICIT Extensions OPTIONAL
+ *)
+  x509_extensions_t_inbound serialize_aliasKeyTBS_extensions
 )
 
 let synth_aliasKeyTBS_payload_t
-  (header_len: asn1_int32)
-  (x': aliasKeyTBS_payload_t' header_len)
-: GTot (aliasKeyTBS_payload_t header_len)
-= { aliasKeyTBS_template     = fst (fst x');
+  (x': aliasKeyTBS_payload_t')
+: GTot (aliasKeyTBS_payload_t)
+= { aliasKeyTBS_version      = fst (fst (fst (fst (fst (fst (fst x'))))));
+    aliasKeyTBS_serialNumber = snd (fst (fst (fst (fst (fst (fst x'))))));
+    aliasKeyTBS_signatureAlg = snd (fst (fst (fst (fst (fst x')))));
+    aliasKeyTBS_issuer       = snd (fst (fst (fst (fst x'))));
+    aliasKeyTBS_validity     = snd (fst (fst (fst x')));
+    aliasKeyTBS_subject      = snd (fst (fst x'));
     aliasKeyTBS_aliasKey_pub = snd (fst x');
     aliasKeyTBS_extensions   = snd x' }
 
 let synth_aliasKeyTBS_payload_t'
-  (header_len: asn1_int32)
-  (x: aliasKeyTBS_payload_t header_len)
-: Tot (x': aliasKeyTBS_payload_t' header_len { x == synth_aliasKeyTBS_payload_t header_len x' })
-= (x.aliasKeyTBS_template,
-   x.aliasKeyTBS_aliasKey_pub),
-   x.aliasKeyTBS_extensions
+  (x: aliasKeyTBS_payload_t)
+: Tot (x': aliasKeyTBS_payload_t' { x == synth_aliasKeyTBS_payload_t x' })
+= ((((((x.aliasKeyTBS_version,
+        x.aliasKeyTBS_serialNumber),
+        x.aliasKeyTBS_signatureAlg),
+        x.aliasKeyTBS_issuer),
+        x.aliasKeyTBS_validity),
+        x.aliasKeyTBS_subject),
+        x.aliasKeyTBS_aliasKey_pub),
+        x.aliasKeyTBS_extensions
 
 let parse_aliasKeyTBS_payload
-  (header_len: asn1_int32)
-: parser _ (aliasKeyTBS_payload_t header_len)
-= parse_flbytes32 header_len
+: parser _ aliasKeyTBS_payload_t
+= parse_x509_version
+  `nondep_then`
+  parse_asn1_TLV_of_type INTEGER
+  `nondep_then`
+  parse_algorithmIdentifier
+  `nondep_then`
+  parse_aliasKeyTBS_issuer
+  `nondep_then`
+  parse_x509_validity
+  `nondep_then`
+  parse_aliasKeyTBS_subject
   `nondep_then`
   parse_subjectPublicKeyInfo
   `nondep_then`
   parse_x509_extensions_TLV serialize_aliasKeyTBS_extensions
   `parse_synth`
-  synth_aliasKeyTBS_payload_t header_len
+  synth_aliasKeyTBS_payload_t
 
 let serialize_aliasKeyTBS_payload
-  (header_len: asn1_int32)
-: serializer (parse_aliasKeyTBS_payload header_len)
+: serializer (parse_aliasKeyTBS_payload)
 = serialize_synth
-  (* p1 *) (parse_flbytes32 header_len
+  (* p1 *) (parse_x509_version
+            `nondep_then`
+            parse_asn1_TLV_of_type INTEGER
+            `nondep_then`
+            parse_algorithmIdentifier
+            `nondep_then`
+            parse_aliasKeyTBS_issuer
+            `nondep_then`
+            parse_x509_validity
+            `nondep_then`
+            parse_aliasKeyTBS_subject
             `nondep_then`
             parse_subjectPublicKeyInfo
             `nondep_then`
             parse_x509_extensions_TLV serialize_aliasKeyTBS_extensions)
-  (* f2 *) (synth_aliasKeyTBS_payload_t header_len)
-  (* s1 *) (serialize_flbytes32 header_len
+  (* f2 *) (synth_aliasKeyTBS_payload_t)
+  (* s1 *) (serialize_x509_version
+            `serialize_nondep_then`
+            serialize_asn1_TLV_of_type INTEGER
+            `serialize_nondep_then`
+            serialize_algorithmIdentifier
+            `serialize_nondep_then`
+            serialize_aliasKeyTBS_issuer
+            `serialize_nondep_then`
+            serialize_x509_validity
+            `serialize_nondep_then`
+            serialize_aliasKeyTBS_subject
             `serialize_nondep_then`
             serialize_subjectPublicKeyInfo
             `serialize_nondep_then`
             serialize_x509_extensions_TLV serialize_aliasKeyTBS_extensions)
-  (* g1 *) (synth_aliasKeyTBS_payload_t' header_len)
+  (* g1 *) (synth_aliasKeyTBS_payload_t')
   (* prf*) ()
 
 let lemma_serialize_aliasKeyTBS_payload_unfold
-  (header_len: asn1_int32)
-  (x: aliasKeyTBS_payload_t header_len)
+  (x: aliasKeyTBS_payload_t)
 : Lemma (
-  serialize_aliasKeyTBS_payload header_len `serialize` x ==
- (serialize_flbytes32 header_len `serialize` x.aliasKeyTBS_template)
+  serialize_aliasKeyTBS_payload `serialize` x ==
+ (serialize_x509_version `serialize` x.aliasKeyTBS_version)
+  `Seq.append`
+ (serialize_asn1_TLV_of_type INTEGER `serialize` x.aliasKeyTBS_serialNumber)
+  `Seq.append`
+ (serialize_algorithmIdentifier `serialize` x.aliasKeyTBS_signatureAlg)
+  `Seq.append`
+ (serialize_aliasKeyTBS_issuer `serialize` x.aliasKeyTBS_issuer)
+  `Seq.append`
+ (serialize_x509_validity `serialize` x.aliasKeyTBS_validity)
+  `Seq.append`
+ (serialize_aliasKeyTBS_subject `serialize` x.aliasKeyTBS_subject)
   `Seq.append`
  (serialize_subjectPublicKeyInfo `serialize` x.aliasKeyTBS_aliasKey_pub)
   `Seq.append`
  (serialize_x509_extensions_TLV serialize_aliasKeyTBS_extensions `serialize` x.aliasKeyTBS_extensions)
 )
-= serialize_nondep_then_eq
-  (* s1 *) (serialize_flbytes32 header_len)
-  (* s2 *) (serialize_subjectPublicKeyInfo)
-  (* in *) (fst (synth_aliasKeyTBS_payload_t' header_len x));
+=
   serialize_nondep_then_eq
-  (* s1 *) (serialize_flbytes32 header_len
+  (* s1 *) (serialize_x509_version)
+  (* s2 *) (serialize_asn1_TLV_of_type INTEGER)
+  (* in *) (fst (fst (fst(fst (fst (fst (synth_aliasKeyTBS_payload_t' x)))))));
+
+  serialize_nondep_then_eq
+  (* s1 *) (serialize_x509_version
+            `serialize_nondep_then`
+            serialize_asn1_TLV_of_type INTEGER)
+  (* s2 *) (serialize_algorithmIdentifier)
+  (* in *) (fst (fst(fst (fst (fst (synth_aliasKeyTBS_payload_t' x))))));
+
+  serialize_nondep_then_eq
+  (* s1 *) (serialize_x509_version
+            `serialize_nondep_then`
+            serialize_asn1_TLV_of_type INTEGER
+            `serialize_nondep_then`
+            serialize_algorithmIdentifier)
+  (* s2 *) (serialize_aliasKeyTBS_issuer)
+  (* in *) (fst (fst (fst (fst (synth_aliasKeyTBS_payload_t' x)))));
+
+  serialize_nondep_then_eq
+  (* s1 *) (serialize_x509_version
+            `serialize_nondep_then`
+            serialize_asn1_TLV_of_type INTEGER
+            `serialize_nondep_then`
+            serialize_algorithmIdentifier
+            `serialize_nondep_then`
+            serialize_aliasKeyTBS_issuer)
+  (* s2 *) (serialize_x509_validity)
+  (* in *) (fst (fst (fst (synth_aliasKeyTBS_payload_t' x))));
+
+  serialize_nondep_then_eq
+  (* s1 *) (serialize_x509_version
+            `serialize_nondep_then`
+            serialize_asn1_TLV_of_type INTEGER
+            `serialize_nondep_then`
+            serialize_algorithmIdentifier
+            `serialize_nondep_then`
+            serialize_aliasKeyTBS_issuer
+            `serialize_nondep_then`
+            serialize_x509_validity)
+  (* s2 *) (serialize_aliasKeyTBS_subject)
+  (* in *) (fst (fst (synth_aliasKeyTBS_payload_t' x)));
+
+  serialize_nondep_then_eq
+  (* s1 *) (serialize_x509_version
+            `serialize_nondep_then`
+            serialize_asn1_TLV_of_type INTEGER
+            `serialize_nondep_then`
+            serialize_algorithmIdentifier
+            `serialize_nondep_then`
+            serialize_aliasKeyTBS_issuer
+            `serialize_nondep_then`
+            serialize_x509_validity
+            `serialize_nondep_then`
+            serialize_aliasKeyTBS_subject)
+  (* s2 *) (serialize_subjectPublicKeyInfo)
+  (* in *) (fst (synth_aliasKeyTBS_payload_t' x));
+
+  serialize_nondep_then_eq
+  (* s1 *) (serialize_x509_version
+            `serialize_nondep_then`
+            serialize_asn1_TLV_of_type INTEGER
+            `serialize_nondep_then`
+            serialize_algorithmIdentifier
+            `serialize_nondep_then`
+            serialize_aliasKeyTBS_issuer
+            `serialize_nondep_then`
+            serialize_x509_validity
+            `serialize_nondep_then`
+            serialize_aliasKeyTBS_subject
             `serialize_nondep_then`
             serialize_subjectPublicKeyInfo)
   (* s2 *) (serialize_x509_extensions_TLV serialize_aliasKeyTBS_extensions)
-  (* in *) (synth_aliasKeyTBS_payload_t' header_len x);
+  (* in *) (synth_aliasKeyTBS_payload_t' x);
+
   serialize_synth_eq
-  (* p1 *) (parse_flbytes32 header_len
+  (* p1 *) (parse_x509_version
+            `nondep_then`
+            parse_asn1_TLV_of_type INTEGER
+            `nondep_then`
+            parse_algorithmIdentifier
+            `nondep_then`
+            parse_aliasKeyTBS_issuer
+            `nondep_then`
+            parse_x509_validity
+            `nondep_then`
+            parse_aliasKeyTBS_subject
             `nondep_then`
             parse_subjectPublicKeyInfo
             `nondep_then`
             parse_x509_extensions_TLV serialize_aliasKeyTBS_extensions)
-  (* f2 *) (synth_aliasKeyTBS_payload_t header_len)
-  (* s1 *) (serialize_flbytes32 header_len
+  (* f2 *) (synth_aliasKeyTBS_payload_t)
+  (* s1 *) (serialize_x509_version
+            `serialize_nondep_then`
+            serialize_asn1_TLV_of_type INTEGER
+            `serialize_nondep_then`
+            serialize_algorithmIdentifier
+            `serialize_nondep_then`
+            serialize_aliasKeyTBS_issuer
+            `serialize_nondep_then`
+            serialize_x509_validity
+            `serialize_nondep_then`
+            serialize_aliasKeyTBS_subject
             `serialize_nondep_then`
             serialize_subjectPublicKeyInfo
             `serialize_nondep_then`
             serialize_x509_extensions_TLV serialize_aliasKeyTBS_extensions)
-  (* g1 *) (synth_aliasKeyTBS_payload_t' header_len)
+  (* g1 *) (synth_aliasKeyTBS_payload_t')
   (* prf*) ()
-  (* in *) x
+  (* in *) (x)
 
-#restart-solver
-#push-options "--z3rlimit 64 --fuel 0 --ifuel 0"
 let length_of_aliasKeyTBS_payload
-  (header_len: asn1_int32)
+  (serialNumber: datatype_of_asn1_type INTEGER)
+  (i_common:  x509_RDN_x520_attribute_string_t COMMON_NAME  IA5_STRING)
+  (i_org:     x509_RDN_x520_attribute_string_t ORGANIZATION IA5_STRING)
+  (i_country: x509_RDN_x520_attribute_string_t COUNTRY      PRINTABLE_STRING)
+  (s_common:  x509_RDN_x520_attribute_string_t COMMON_NAME  IA5_STRING)
+  (s_org:     x509_RDN_x520_attribute_string_t ORGANIZATION IA5_STRING)
+  (s_country: x509_RDN_x520_attribute_string_t COUNTRY      PRINTABLE_STRING)
   (ku: key_usage_payload_t)
   (version: datatype_of_asn1_type INTEGER)
 : GTot (nat)
-= v header_len +
+= length_of_x509_version () +
+  length_of_asn1_primitive_TLV serialNumber +
+  length_of_algorithmIdentifier () +
+  length_of_aliasKeyTBS_issuer i_common i_org i_country +
+  length_of_x509_validity () +
+  length_of_aliasKeyTBS_subject s_common s_org s_country +
   length_of_subjectPublicKeyInfo +
   length_of_x509_extensions (length_of_aliasKeyTBS_extensions ku version)
 
 let len_of_aliasKeyTBS_payload
-  (header_len: asn1_int32)
+  (serialNumber: datatype_of_asn1_type INTEGER)
+  (i_common:  x509_RDN_x520_attribute_string_t COMMON_NAME  IA5_STRING)
+  (i_org:     x509_RDN_x520_attribute_string_t ORGANIZATION IA5_STRING)
+  (i_country: x509_RDN_x520_attribute_string_t COUNTRY      PRINTABLE_STRING)
+  (s_common:  x509_RDN_x520_attribute_string_t COMMON_NAME  IA5_STRING)
+  (s_org:     x509_RDN_x520_attribute_string_t ORGANIZATION IA5_STRING)
+  (s_country: x509_RDN_x520_attribute_string_t COUNTRY      PRINTABLE_STRING)
   (ku: key_usage_payload_t)
   (version: datatype_of_asn1_type INTEGER
-            { length_of_aliasKeyTBS_payload header_len ku version
+            { length_of_aliasKeyTBS_payload
+                serialNumber
+                i_common i_org i_country
+                s_common s_org s_country
+                ku version
               <= asn1_value_length_max_of_type SEQUENCE })
 : Tot (len: asn1_TLV_int32_of_type SEQUENCE
-            { v len == length_of_aliasKeyTBS_payload header_len ku version })
-= header_len +
+            { v len == length_of_aliasKeyTBS_payload
+                         serialNumber
+                         i_common i_org i_country
+                         s_common s_org s_country
+                         ku version })
+= len_of_x509_version () +
+  len_of_asn1_primitive_TLV serialNumber +
+  len_of_algorithmIdentifier () +
+  len_of_aliasKeyTBS_issuer i_common i_org i_country +
+  len_of_x509_validity () +
+  len_of_aliasKeyTBS_subject s_common s_org s_country +
   len_of_subjectPublicKeyInfo +
   len_of_x509_extensions (len_of_aliasKeyTBS_extensions ku version)
 
+#restart-solver
+#push-options "--z3rlimit 512"
 let lemma_serialize_aliasKeyTBS_payload_size
-  (header_len: asn1_int32)
-  (x: aliasKeyTBS_payload_t header_len)
+  (x: aliasKeyTBS_payload_t)
 : Lemma (
   let riot_version = RIoT.X509.Extension.(x.aliasKeyTBS_extensions.aliasKeyTBS_extensions_riot.x509_extValue_riot.riot_version) in
   let ku = (snd x.aliasKeyTBS_extensions.aliasKeyTBS_extensions_key_usage) in
   (* unfold *)
-  length_of_opaque_serialization (serialize_aliasKeyTBS_payload header_len)              x ==
-  length_of_opaque_serialization (serialize_flbytes32 header_len)                x.aliasKeyTBS_template     +
-  length_of_opaque_serialization (serialize_subjectPublicKeyInfo)   x.aliasKeyTBS_aliasKey_pub +
+  length_of_opaque_serialization (serialize_aliasKeyTBS_payload) x ==
+  length_of_opaque_serialization (serialize_x509_version)             x.aliasKeyTBS_version      +
+  length_of_opaque_serialization (serialize_asn1_TLV_of_type INTEGER) x.aliasKeyTBS_serialNumber +
+  length_of_opaque_serialization (serialize_algorithmIdentifier)      x.aliasKeyTBS_signatureAlg +
+  length_of_opaque_serialization (serialize_aliasKeyTBS_issuer)       x.aliasKeyTBS_issuer     +
+  length_of_opaque_serialization (serialize_x509_validity)            x.aliasKeyTBS_validity     +
+  length_of_opaque_serialization (serialize_aliasKeyTBS_subject)      x.aliasKeyTBS_subject     +
+  length_of_opaque_serialization (serialize_subjectPublicKeyInfo)     x.aliasKeyTBS_aliasKey_pub +
   length_of_opaque_serialization (serialize_x509_extensions_TLV
-                                  serialize_aliasKeyTBS_extensions) x.aliasKeyTBS_extensions /\
+                                  serialize_aliasKeyTBS_extensions)   x.aliasKeyTBS_extensions /\
   (* exact size *)
-  length_of_opaque_serialization (serialize_aliasKeyTBS_payload header_len)            x
-  == length_of_aliasKeyTBS_payload header_len ku riot_version
-  (* upper bound *)
-  // length_of_opaque_serialization (serialize_aliasKeyTBS header_len)            x
-  // <= v header_len + 44 + (6 + (6 + 117))
+  length_of_opaque_serialization (serialize_aliasKeyTBS_payload) x
+  == length_of_aliasKeyTBS_payload
+       x.aliasKeyTBS_serialNumber
+       (get_RDN_x520_attribute_string x.aliasKeyTBS_issuer.aliasKeyTBS_issuer_Common)
+       (get_RDN_x520_attribute_string x.aliasKeyTBS_issuer.aliasKeyTBS_issuer_Organization)
+       (get_RDN_x520_attribute_string x.aliasKeyTBS_issuer.aliasKeyTBS_issuer_Country)
+       (get_RDN_x520_attribute_string x.aliasKeyTBS_subject.aliasKeyTBS_subject_Common)
+       (get_RDN_x520_attribute_string x.aliasKeyTBS_subject.aliasKeyTBS_subject_Organization)
+       (get_RDN_x520_attribute_string x.aliasKeyTBS_subject.aliasKeyTBS_subject_Country)
+       ku
+       riot_version
 )
-= lemma_serialize_aliasKeyTBS_payload_unfold header_len x;
-    (* + v header_len *)
-    (* + 44 *)
+= lemma_serialize_aliasKeyTBS_payload_unfold x;
+    lemma_serialize_x509_version_size_exact x.aliasKeyTBS_version;
+    lemma_serialize_asn1_integer_TLV_size x.aliasKeyTBS_serialNumber;
+    lemma_serialize_algorithmIdentifier_size_exact x.aliasKeyTBS_signatureAlg;
+    lemma_serialize_aliasKeyTBS_issuer_size_exact x.aliasKeyTBS_issuer;
+    lemma_serialize_x509_validity_size_exact x.aliasKeyTBS_validity;
+    lemma_serialize_aliasKeyTBS_subject_size_exact x.aliasKeyTBS_subject;
     lemma_serialize_subjectPublicKeyInfo_size_exact x.aliasKeyTBS_aliasKey_pub;
-    (* + (6) *)
     lemma_serialize_x509_extensions_TLV_size serialize_aliasKeyTBS_extensions x.aliasKeyTBS_extensions;
-      (* + (6 + 117) / + |riot_veriosn| + 113 *)
       lemma_serialize_aliasKeyTBS_extensions_size_exact x.aliasKeyTBS_extensions
 #pop-options
 
-
 let aliasKeyTBS_t
-  (header_len: asn1_int32)
-= inbound_sequence_value_of (serialize_aliasKeyTBS_payload header_len)
+= inbound_sequence_value_of (serialize_aliasKeyTBS_payload)
 
 let parse_aliasKeyTBS
-  (header_len: asn1_int32)
-: parser (parse_asn1_envelop_tag_with_TLV_kind SEQUENCE) (aliasKeyTBS_t header_len)
+: parser (parse_asn1_envelop_tag_with_TLV_kind SEQUENCE) (aliasKeyTBS_t)
 =
-  aliasKeyTBS_t header_len
+  aliasKeyTBS_t
   `coerce_parser`
-  parse_asn1_sequence_TLV (serialize_aliasKeyTBS_payload header_len)
+  parse_asn1_sequence_TLV (serialize_aliasKeyTBS_payload)
 
 let serialize_aliasKeyTBS
-  (header_len: asn1_int32)
-: serializer (parse_aliasKeyTBS header_len)
+: serializer (parse_aliasKeyTBS)
 = coerce_parser_serializer
-    (parse_aliasKeyTBS header_len)
-    (serialize_asn1_sequence_TLV (serialize_aliasKeyTBS_payload header_len))
+    (parse_aliasKeyTBS)
+    (serialize_asn1_sequence_TLV (serialize_aliasKeyTBS_payload))
     ()
 
 let lemma_serialize_aliasKeyTBS_unfold
-  (header_len: asn1_int32)
-  (x: aliasKeyTBS_t header_len)
-: Lemma ( predicate_serialize_asn1_sequence_TLV_unfold (serialize_aliasKeyTBS_payload header_len) x )
-= lemma_serialize_asn1_sequence_TLV_unfold (serialize_aliasKeyTBS_payload header_len) x
+  (x: aliasKeyTBS_t)
+: Lemma ( predicate_serialize_asn1_sequence_TLV_unfold (serialize_aliasKeyTBS_payload) x )
+= lemma_serialize_asn1_sequence_TLV_unfold (serialize_aliasKeyTBS_payload) x
 
 let lemma_serialize_aliasKeyTBS_size
-  (header_len: asn1_int32)
-  (x: aliasKeyTBS_t header_len)
-: Lemma ( predicate_serialize_asn1_sequence_TLV_size (serialize_aliasKeyTBS_payload header_len) x )
-= lemma_serialize_asn1_sequence_TLV_size (serialize_aliasKeyTBS_payload header_len) x
+  (x: aliasKeyTBS_t)
+: Lemma ( predicate_serialize_asn1_sequence_TLV_size (serialize_aliasKeyTBS_payload) x )
+= lemma_serialize_asn1_sequence_TLV_size (serialize_aliasKeyTBS_payload) x
 
-#push-options "--z3rlimit 64 --fuel 0 --ifuel 0"
 let length_of_aliasKeyTBS
-  (header_len: asn1_int32)
+  (serialNumber: datatype_of_asn1_type INTEGER)
+  (i_common:  x509_RDN_x520_attribute_string_t COMMON_NAME  IA5_STRING)
+  (i_org:     x509_RDN_x520_attribute_string_t ORGANIZATION IA5_STRING)
+  (i_country: x509_RDN_x520_attribute_string_t COUNTRY      PRINTABLE_STRING)
+  (s_common:  x509_RDN_x520_attribute_string_t COMMON_NAME  IA5_STRING)
+  (s_org:     x509_RDN_x520_attribute_string_t ORGANIZATION IA5_STRING)
+  (s_country: x509_RDN_x520_attribute_string_t COUNTRY      PRINTABLE_STRING)
   (ku: key_usage_payload_t)
   (version: datatype_of_asn1_type INTEGER
-            { length_of_aliasKeyTBS_payload header_len ku version
+            { length_of_aliasKeyTBS_payload
+                serialNumber
+                i_common i_org i_country
+                s_common s_org s_country
+                ku version
               <= asn1_value_length_max_of_type SEQUENCE })
 : GTot (asn1_TLV_length_of_type SEQUENCE)
-= length_of_TLV SEQUENCE (length_of_aliasKeyTBS_payload header_len ku version)
-
-let len_of_aliasKeyTBS
-  (header_len: asn1_int32)
-  (ku: key_usage_payload_t)
-  (version: datatype_of_asn1_type INTEGER
-            { length_of_aliasKeyTBS_payload header_len ku version
-              <= asn1_value_length_max_of_type SEQUENCE })
-: Tot (len: asn1_TLV_int32_of_type SEQUENCE
-            { v len == length_of_aliasKeyTBS header_len ku version })
-= len_of_TLV SEQUENCE (len_of_aliasKeyTBS_payload header_len ku version)
-#pop-options
+= length_of_TLV
+    (SEQUENCE)
+    (length_of_aliasKeyTBS_payload
+      serialNumber
+      i_common i_org i_country
+      s_common s_org s_country
+      ku version)
 
 #restart-solver
-#push-options "--z3rlimit 64 --fuel 0 --ifuel 0"
+let len_of_aliasKeyTBS
+  (serialNumber: datatype_of_asn1_type INTEGER)
+  (i_common:  x509_RDN_x520_attribute_string_t COMMON_NAME  IA5_STRING)
+  (i_org:     x509_RDN_x520_attribute_string_t ORGANIZATION IA5_STRING)
+  (i_country: x509_RDN_x520_attribute_string_t COUNTRY      PRINTABLE_STRING)
+  (s_common:  x509_RDN_x520_attribute_string_t COMMON_NAME  IA5_STRING)
+  (s_org:     x509_RDN_x520_attribute_string_t ORGANIZATION IA5_STRING)
+  (s_country: x509_RDN_x520_attribute_string_t COUNTRY      PRINTABLE_STRING)
+  (ku: key_usage_payload_t)
+  (version: datatype_of_asn1_type INTEGER
+            { length_of_aliasKeyTBS_payload
+                serialNumber
+                i_common i_org i_country
+                s_common s_org s_country
+                ku version
+              <= asn1_value_length_max_of_type SEQUENCE })
+// : Tot (len: asn1_TLV_length_of_type SEQUENCE
+//              { v len == length_of_aliasKeyTBS
+//                           serialNumber
+//                           i_common i_org i_country
+//                           s_common s_org s_country
+//                           ku version })
+= len_of_TLV
+    (SEQUENCE)
+    (len_of_aliasKeyTBS_payload
+      serialNumber
+      i_common i_org i_country
+      s_common s_org s_country
+      ku version)
+
+#restart-solver
+#push-options "--z3rlimit 512"
 let lemma_serialize_aliasKeyTBS_size_exact
-  (header_len: asn1_int32)
-  (x: aliasKeyTBS_t header_len)
+  (x: aliasKeyTBS_t)
 : Lemma (
   let riot_version = RIoT.X509.Extension.(x.aliasKeyTBS_extensions.aliasKeyTBS_extensions_riot.x509_extValue_riot.riot_version) in
   let ku = (snd x.aliasKeyTBS_extensions.aliasKeyTBS_extensions_key_usage) in
-  let _ = lemma_serialize_aliasKeyTBS_payload_size header_len x in
+  let _ = lemma_serialize_aliasKeyTBS_payload_size x in
   (* exact size *)
-  length_of_opaque_serialization (serialize_aliasKeyTBS header_len) x
-  == length_of_aliasKeyTBS header_len ku riot_version
-  (* upper bound *)
-  // length_of_opaque_serialization (serialize_aliasKeyTBS header_len) x
-  // <= (6 + v header_len + 44 + (6 + (6 + 117)))
+  length_of_opaque_serialization (serialize_aliasKeyTBS) x
+  == length_of_aliasKeyTBS
+       x.aliasKeyTBS_serialNumber
+       (get_RDN_x520_attribute_string x.aliasKeyTBS_issuer.aliasKeyTBS_issuer_Common)
+       (get_RDN_x520_attribute_string x.aliasKeyTBS_issuer.aliasKeyTBS_issuer_Organization)
+       (get_RDN_x520_attribute_string x.aliasKeyTBS_issuer.aliasKeyTBS_issuer_Country)
+       (get_RDN_x520_attribute_string x.aliasKeyTBS_subject.aliasKeyTBS_subject_Common)
+       (get_RDN_x520_attribute_string x.aliasKeyTBS_subject.aliasKeyTBS_subject_Organization)
+       (get_RDN_x520_attribute_string x.aliasKeyTBS_subject.aliasKeyTBS_subject_Country)
+       ku
+       riot_version
 )
-= lemma_serialize_aliasKeyTBS_size header_len x;
-    lemma_serialize_aliasKeyTBS_payload_size header_len x
+= lemma_serialize_aliasKeyTBS_size x;
+    lemma_serialize_aliasKeyTBS_payload_size x
 #pop-options
-
 
 (* low *)
 let serialize32_aliasKeyTBS_payload_backwards
-  (header_len: asn1_int32)
-: serializer32_backwards (serialize_aliasKeyTBS_payload header_len)
+: serializer32_backwards (serialize_aliasKeyTBS_payload)
 = serialize32_synth_backwards
-  (* s1 *) (serialize32_flbytes32_backwards header_len
+  (* s1 *) (serialize32_x509_version_backwards
+            `serialize32_nondep_then_backwards`
+            serialize32_asn1_TLV_backwards_of_type INTEGER
+            `serialize32_nondep_then_backwards`
+            serialize32_algorithmIdentifier_backwards
+            `serialize32_nondep_then_backwards`
+            serialize32_aliasKeyTBS_issuer_backwards
+            `serialize32_nondep_then_backwards`
+            serialize32_x509_validity_backwards
+            `serialize32_nondep_then_backwards`
+            serialize32_aliasKeyTBS_subject_backwards
             `serialize32_nondep_then_backwards`
             serialize32_subjectPublicKeyInfo_backwards
             `serialize32_nondep_then_backwards`
             serialize32_x509_extensions_TLV_backwards serialize32_aliasKeyTBS_extensions_backwards)
-  (* f2 *) (synth_aliasKeyTBS_payload_t  header_len)
-  (* g1 *) (synth_aliasKeyTBS_payload_t' header_len)
-  (* g1'*) (synth_aliasKeyTBS_payload_t' header_len)
+  (* f2 *) (synth_aliasKeyTBS_payload_t)
+  (* g1 *) (synth_aliasKeyTBS_payload_t')
+  (* g1'*) (synth_aliasKeyTBS_payload_t')
   (* prf*) ()
 
 let serialize32_aliasKeyTBS_backwards
-  (header_len: asn1_int32)
-: serializer32_backwards (serialize_aliasKeyTBS header_len)
+: serializer32_backwards (serialize_aliasKeyTBS)
 = coerce_serializer32_backwards
-  (* s2 *) (serialize_aliasKeyTBS header_len)
+  (* s2 *) (serialize_aliasKeyTBS)
   (* s32*) (serialize32_asn1_sequence_TLV_backwards
-             (serialize32_aliasKeyTBS_payload_backwards header_len))
+             (serialize32_aliasKeyTBS_payload_backwards))
   (* prf*) ()
 
 
 (* helpers *)
 #restart-solver
-#push-options "--z3rlimit 64 --fuel 0 --ifuel 0"
 let x509_get_AliasKeyTBS
-  (header_len: asn1_int32)
-  (aliasKeyTBS_template: B32.lbytes32 header_len)
+  (crt_version: x509_version_t)
+  (serialNumber: datatype_of_asn1_type INTEGER)
+  (i_common:  x509_RDN_x520_attribute_string_t COMMON_NAME  IA5_STRING)
+  (i_org:     x509_RDN_x520_attribute_string_t ORGANIZATION IA5_STRING)
+  (i_country: x509_RDN_x520_attribute_string_t COUNTRY      PRINTABLE_STRING
+              { length_of_aliasKeyTBS_issuer_payload i_common i_org i_country
+                <= asn1_value_length_max_of_type SEQUENCE })
+  (notBefore: datatype_of_asn1_type Generalized_Time)
+  (notAfter : datatype_of_asn1_type Generalized_Time)
+  (s_common:  x509_RDN_x520_attribute_string_t COMMON_NAME  IA5_STRING)
+  (s_org:     x509_RDN_x520_attribute_string_t ORGANIZATION IA5_STRING)
+  (s_country: x509_RDN_x520_attribute_string_t COUNTRY      PRINTABLE_STRING)
   (ku: key_usage_payload_t)
   (version: datatype_of_asn1_type INTEGER
-            { length_of_aliasKeyTBS_payload header_len ku version
+            { length_of_aliasKeyTBS_payload
+                serialNumber
+                i_common i_org i_country
+                s_common s_org s_country
+                ku version
               <= asn1_value_length_max_of_type SEQUENCE })
   (fwid: B32.lbytes32 32ul)
   (deviceIDPub: B32.lbytes32 32ul)
   (aliasKeyPub: B32.lbytes32 32ul)
-: Tot (aliasKeyTBS_t header_len)
+: Tot (aliasKeyTBS_t)
 =
-  let aliasKeyTBS_extensions = x509_get_aliasKeyTBS_extensions
-                                 ku
-                                 version
-                                 fwid
-                                 deviceIDPub in
-  (* Prf *) lemma_serialize_aliasKeyTBS_extensions_size_exact aliasKeyTBS_extensions;
+  let signatureAlg: algorithmIdentifier_t = x509_get_algorithmIdentifier () in
+  (* Prf *) lemma_serialize_algorithmIdentifier_size_exact signatureAlg;
+
+  let issuer: aliasKeyTBS_issuer_t = x509_get_aliasKeyTBS_issuer
+    #(dfst (i_common <: datatype_of_asn1_type IA5_STRING))
+    (dsnd (i_common <: datatype_of_asn1_type IA5_STRING))
+    #(dfst (i_org <: datatype_of_asn1_type IA5_STRING))
+    (dsnd (i_org <: datatype_of_asn1_type IA5_STRING))
+    #(dfst (i_country <: datatype_of_asn1_type PRINTABLE_STRING))
+    (dsnd (i_country <: datatype_of_asn1_type PRINTABLE_STRING)) in
+  (* Prf *) lemma_serialize_aliasKeyTBS_issuer_size_exact issuer;
+
+  let validity: x509_validity_t = x509_get_validity
+                                    notBefore
+                                    notAfter in
+  (* Prf *) lemma_serialize_x509_validity_size_exact validity;
+
+  let subject: aliasKeyTBS_subject_t = x509_get_aliasKeyTBS_subject
+    #(dfst (s_common <: datatype_of_asn1_type IA5_STRING))
+    (dsnd (s_common <: datatype_of_asn1_type IA5_STRING))
+    #(dfst (s_org <: datatype_of_asn1_type IA5_STRING))
+    (dsnd (s_org <: datatype_of_asn1_type IA5_STRING))
+    #(dfst (s_country <: datatype_of_asn1_type PRINTABLE_STRING))
+    (dsnd (s_country <: datatype_of_asn1_type PRINTABLE_STRING)) in
+  (* Prf *) lemma_serialize_aliasKeyTBS_subject_size_exact subject;
 
   let aliasKeyPubInfo = x509_get_subjectPublicKeyInfo
                            aliasKeyPub in
   (* Prf *) lemma_serialize_subjectPublicKeyInfo_size_exact aliasKeyPubInfo;
 
-  let aliasKeyTBS: aliasKeyTBS_payload_t header_len = {
-    aliasKeyTBS_template       = aliasKeyTBS_template;
+  let extensions = x509_get_aliasKeyTBS_extensions
+                                 ku
+                                 version
+                                 fwid
+                                 deviceIDPub in
+  (* Prf *) lemma_serialize_aliasKeyTBS_extensions_size_exact extensions;
+
+  let aliasKeyTBS: aliasKeyTBS_payload_t = {
+    aliasKeyTBS_version        = crt_version;
+    aliasKeyTBS_serialNumber   = serialNumber;
+    aliasKeyTBS_signatureAlg   = signatureAlg;
+    aliasKeyTBS_issuer         = issuer;
+    aliasKeyTBS_validity       = validity;
+    aliasKeyTBS_subject        = subject;
     aliasKeyTBS_aliasKey_pub   = aliasKeyPubInfo;
-    aliasKeyTBS_extensions     = aliasKeyTBS_extensions
+    aliasKeyTBS_extensions     = extensions
   } in
-  (* Prf *) lemma_serialize_aliasKeyTBS_payload_unfold header_len aliasKeyTBS;
-  (* Prf *) lemma_serialize_aliasKeyTBS_payload_size   header_len aliasKeyTBS;
-  (* Prf *) (**) lemma_serialize_flbytes32_size header_len aliasKeyTBS.aliasKeyTBS_template;
+  (* Prf *) lemma_serialize_aliasKeyTBS_payload_unfold aliasKeyTBS;
+  (* Prf *) lemma_serialize_aliasKeyTBS_payload_size   aliasKeyTBS;
+  (* Prf *) (**) lemma_serialize_x509_version_size_exact crt_version;
+  (* Prf *) (**) lemma_serialize_asn1_integer_TLV_size serialNumber;
 
 (*return*) aliasKeyTBS
