src/riot/x509/X509.BasicFields.Validity.fst
@@ -8,3 +8,204 @@ open ASN1.Low
 open X509.Base
 
 open FStar.Integers
+
+(*
+ 4.1.2.5.  Validity
+
+   The certificate validity period is the time interval during which the
+   CA warrants that it will maintain information about the status of the
+   certificate.  The field is represented as a SEQUENCE of two dates:
+   the date on which the certificate validity period begins (notBefore)
+   and the date on which the certificate validity period ends
+   (notAfter).  Both notBefore and notAfter may be encoded as UTCTime or
+   GeneralizedTime.
+
+   CAs conforming to this profile MUST always encode certificate
+   validity dates through the year 2049 as UTCTime; certificate validity
+   dates in 2050 or later MUST be encoded as GeneralizedTime.
+   Conforming applications MUST be able to process validity dates that
+   are encoded in either UTCTime or GeneralizedTime.
+
+   The validity period for a certificate is the period of time from
+   notBefore through notAfter, inclusive.
+
+   In some situations, devices are given certificates for which no good
+   expiration date can be assigned.  For example, a device could be
+   issued a certificate that binds its model and serial number to its
+   public key; such a certificate is intended to be used for the entire
+   lifetime of the device.
+
+   To indicate that a certificate has no well-defined expiration date,
+   the notAfter SHOULD be assigned the GeneralizedTime value of
+   99991231235959Z.
+*)
+
+#set-options "--z3rlimit 32 --fuel 0 --ifuel 0"
+
+type x509_validity_payload_t: Type = {
+  notBefore: generalized_time_t;
+  notAfter: generalized_time_t
+}
+
+let x509_validity_payload_t' = (
+  generalized_time_t `tuple2`
+  generalized_time_t
+)
+
+let synth_x509_validity_payload
+  (x: x509_validity_payload_t')
+: GTot (x509_validity_payload_t)
+= { notBefore = fst x;
+    notAfter  = snd x }
+
+let synth_x509_validity_payload'
+  (x: x509_validity_payload_t)
+: Tot (x': x509_validity_payload_t'
+           { x == synth_x509_validity_payload x' })
+= ( x.notBefore,
+    x.notAfter )
+
+let parse_x509_validity_payload
+: parser _ x509_validity_payload_t
+= parse_asn1_TLV_of_type Generalized_Time
+  `nondep_then`
+  parse_asn1_TLV_of_type Generalized_Time
+  `parse_synth`
+  synth_x509_validity_payload
+
+let serialize_x509_validity_payload
+: serializer parse_x509_validity_payload
+= serialize_synth
+  (* p1 *) (parse_asn1_TLV_of_type Generalized_Time
+            `nondep_then`
+            parse_asn1_TLV_of_type Generalized_Time)
+  (* f2 *) (synth_x509_validity_payload)
+  (* s1 *) (serialize_asn1_TLV_of_type Generalized_Time
+            `serialize_nondep_then`
+            serialize_asn1_TLV_of_type Generalized_Time)
+  (* g1 *) (synth_x509_validity_payload')
+  (* prf*) ()
+
+let lemma_x509_validity_payload_unfold
+  (x: x509_validity_payload_t)
+: Lemma (
+  serialize_x509_validity_payload `serialize` x ==
+ (serialize_asn1_TLV_of_type Generalized_Time `serialize` x.notBefore)
+  `Seq.append`
+ (serialize_asn1_TLV_of_type Generalized_Time `serialize` x.notAfter)
+)
+= serialize_nondep_then_eq
+  (* s1 *) (serialize_asn1_TLV_of_type Generalized_Time)
+  (* s2 *) (serialize_asn1_TLV_of_type Generalized_Time)
+  (* in *) (synth_x509_validity_payload' x);
+  serialize_synth_eq
+  (* p1 *) (parse_asn1_TLV_of_type Generalized_Time
+            `nondep_then`
+            parse_asn1_TLV_of_type Generalized_Time)
+  (* f2 *) (synth_x509_validity_payload)
+  (* s1 *) (serialize_asn1_TLV_of_type Generalized_Time
+            `serialize_nondep_then`
+            serialize_asn1_TLV_of_type Generalized_Time)
+  (* g1 *) (synth_x509_validity_payload')
+  (* prf*) ()
+  (* in *) (x)
+
+let length_of_x509_validity_payload ()
+: GTot (asn1_value_length_of_type SEQUENCE)
+= 30
+
+noextract inline_for_extraction
+let len_of_x509_validity_payload ()
+: Tot (len: asn1_value_int32_of_type SEQUENCE
+            { v len == length_of_x509_validity_payload () })
+= 30ul
+
+let lemma_x509_validity_payload_size
+  (x: x509_validity_payload_t)
+: Lemma (
+  length_of_opaque_serialization serialize_x509_validity_payload x ==
+  length_of_opaque_serialization (serialize_asn1_TLV_of_type Generalized_Time) x.notBefore +
+  length_of_opaque_serialization (serialize_asn1_TLV_of_type Generalized_Time) x.notAfter /\
+  length_of_opaque_serialization serialize_x509_validity_payload x ==
+  length_of_x509_validity_payload ()
+)
+= lemma_x509_validity_payload_unfold x
+
+
+let x509_validity_t: Type
+= inbound_sequence_value_of serialize_x509_validity_payload
+
+let parse_x509_validity
+: parser (parse_asn1_envelop_tag_with_TLV_kind SEQUENCE) (x509_validity_t)
+= x509_validity_t
+  `coerce_parser`
+  parse_asn1_sequence_TLV
+  (**) (serialize_x509_validity_payload)
+
+let serialize_x509_validity
+: serializer (parse_x509_validity)
+= coerce_parser_serializer
+    (parse_x509_validity)
+    (serialize_asn1_sequence_TLV
+    (**) (serialize_x509_validity_payload))
+    ()
+
+let lemma_serialize_x509_validity_unfold
+  (x: x509_validity_t)
+: Lemma ( predicate_serialize_asn1_sequence_TLV_unfold serialize_x509_validity_payload x )
+= lemma_serialize_asn1_sequence_TLV_unfold serialize_x509_validity_payload x
+
+let lemma_serialize_x509_validity_size
+  (x: x509_validity_t)
+: Lemma ( predicate_serialize_asn1_sequence_TLV_size serialize_x509_validity_payload x )
+= lemma_serialize_asn1_sequence_TLV_size serialize_x509_validity_payload x
+
+let length_of_x509_validity ()
+: GTot (asn1_TLV_length_of_type SEQUENCE)
+= 32
+
+let len_of_x509_validity ()
+: Tot (len: asn1_TLV_int32_of_type SEQUENCE
+            { v len == length_of_x509_validity () })
+= 32ul
+
+let lemma_serialize_x509_validity_size_exact
+  (x: x509_validity_t)
+: Lemma (
+  length_of_opaque_serialization serialize_x509_validity x ==
+  length_of_x509_validity ()
+)
+= lemma_serialize_x509_validity_size x
+
+noextract inline_for_extraction
+let serialize32_x509_validity_payload_backwards
+: serializer32_backwards (serialize_x509_validity_payload)
+= serialize32_synth_backwards
+  (* s32 *) (serialize32_asn1_TLV_backwards_of_type Generalized_Time
+             `serialize32_nondep_then_backwards`
+             serialize32_asn1_TLV_backwards_of_type Generalized_Time)
+  (* f2 *) (synth_x509_validity_payload)
+  (* g1 *) (synth_x509_validity_payload')
+  (* g1'*) (synth_x509_validity_payload')
+  (* prf*) ()
+
+noextract inline_for_extraction
+let serialize32_x509_validity_backwards
+: serializer32_backwards (serialize_x509_validity)
+= coerce_serializer32_backwards
+    (serialize_x509_validity)
+    (serialize32_asn1_sequence_TLV_backwards
+    (**) (serialize32_x509_validity_payload_backwards))
+    ()
+
+let x509_get_validity
+  (notBefore: datatype_of_asn1_type Generalized_Time)
+  (notAfter : datatype_of_asn1_type Generalized_Time)
+: Tot (x509_validity_t)
+=
+  let validity: x509_validity_payload_t = {
+      notBefore = notBefore;
+      notAfter  = notAfter
+  } in
+
+(* return *) validity
